Notazione

MasterThesis/LOOP/Interpreter.lean
@@ -4,13 +4,13 @@ namespace LOOP
 
 open LOOP.com
 
-def eval (P : com) (s : store) : store :=
+def eval (P : com) (σ : store) : store :=
   match P with
-  | SKIP    => s
-  | ZER x   => store.update x 0 s
-  | ASN x y => store.update x (s y) s
-  | INC x   => store.update x ((s x) + 1) s
-  | SEQ P Q => (eval Q) (eval P s)
-  | FOR x P => Nat.iterate (fun s' => (eval P s')) (s x) s
+  | SKIP    => σ
+  | ZER x   => store.update x 0 σ
+  | ASN x y => store.update x (σ y) σ
+  | INC x   => store.update x ((σ x) + 1) σ
+  | SEQ P Q => (eval Q) (eval P σ)
+  | FOR x P => (fun σ' => (eval P σ'))^[σ x] σ
 
 end LOOP
